\documentclass{homework}

\title{Homework 11}
\author{Kevin Evans}
\studentid{11571810}
\date{November 11, 2020}
\setclass{Math}{301}
\usepackage{amssymb}
\usepackage{mathtools}

\usepackage{amsthm}
\usepackage{amsmath}
\usepackage{slashed}
\usepackage{relsize}
\usepackage{threeparttable}
\usepackage{float}
\usepackage{booktabs}
\usepackage{boldline}
\usepackage{changepage}
\usepackage{physics}
\usepackage[inter-unit-product =\cdot]{siunitx}
\usepackage{setspace}

\usepackage[makeroom]{cancel}
%\usepackage{pgfplots}

\usepackage{enumitem}
\usepackage{times}
\usepackage{multirow}

\usepackage{amsthm}
\newtheorem*{prop}{Proposition}

\renewcommand\qedsymbol{$\blacksquare$}

\begin{document}
	\maketitle
	
	\begin{enumerate}
		\item \begin{minipage}[t]{\linewidth}
			\begin{prop}
				For a positive integer $n$, \begin{align*}
					\frac{1}{1 \cdot 2} + \frac{1}{2 \cdot 3} + \frac{1}{3 \cdot 4} + \dots + \frac{1}{n(n+1)} = 1 - \frac{1}{n+1}
				\end{align*}
			\end{prop}
			\begin{proof} This will be proven with induction using a base case of $n=1$.
				\begin{enumerate}
					\item[(1)] For $n=1$, it is true that \[\frac{1}{1(1+2)} = 1 - \frac{1}{1+1} \]
					\item[(2)] Suppose it is true $$S(k) = \sum_{i=1}^k \frac{1}{i(i+1)} = 1 - \frac{1}{k+1}$$
					Then for the $k+1$ term, \begin{align*}
						S(k+1) & = \sum_{i=1}^{k+1} \frac{1}{i(i+1)} \\
							& = \sum_{i=1}^k \frac{1}{i(i+1)} + \frac{1}{(k+1)(k+2)} \\
							& = 1 - \frac{1}{k+1} + \frac{1}{(k+1)(k+2)} && \text{(ind. hyp.)}\\
							& = 1 - \frac{k+2}{(k+1)(k+2)} + \frac{1}{(k+1)(k+2)} \\
							& = 1 - \frac{k+1}{(k+1)(k+2)} \\
							& = 1 - \frac{1}{(k+1) + 1}
					\end{align*}
					We have shown $S(k+1)$ to be true and it follows that all $S(n)$ must be true.
				\end{enumerate}
			\end{proof}
		\end{minipage}
	
		\item \begin{minipage}[t]{\linewidth}
			\begin{prop} For every $n \in \mathbb{Z}_{>0}$, 
					$$\sum_{i=1}^n \frac{1}{i^2} \le 2 - \frac{1}{n}$$
			\end{prop}
			\begin{proof} This will be proven with strong induction and a base case of $n=1$.
				\begin{enumerate}
					\item[(1)] For $n=1$, it is true that
						$$1 \le 1$$
						
					\item[(2)] Suppose the true statement $S_k$: 
						$$\sum_{i=1}^k \frac{1}{i^2} \le 2 - \frac{1}{k}$$
						If we consider the next statement in sequence, $S_{k+1}$, \begin{align*}
							\sum_{i=1}^{k+1} \frac{1}{i^2}  & =\sum_{i=1}^{k} \frac{1}{i^2} + \frac{1}{(k+1)^2}
							\intertext{From the inductive hypothesis and by rearranging,}
							\sum_{i=1}^{k} \frac{1}{i^2}  + \frac{1}{(k+1)^2} & \le 2 - \frac{1}{k} + \frac{1}{(k+1)^2}
							\intertext{It is evident that for all positive $k$, as $1/(k+1)^2 < 1/(k+1)$,}
							-\frac{1}{k} + \frac{1}{(k+1)^2} & \le -\frac{1}{k+1}
							\intertext{And as the $\le$ relation is transitive, the inequality of $S_{k+1}$ is also true as}
							\sum_{i=1}^{k+1} \frac{1}{i^2}  & \le 2 - \frac{1}{k + 1}
						\end{align*}
						Therefore this proposition is true for all positive integers.
				\end{enumerate}
			\end{proof}
		\end{minipage}
		
		\item \begin{minipage}[t]{\linewidth}
			\begin{prop} For the Fibonacci sequence $F_n$, 
				\[ \sum_{i=1}^n F_i = F_{n+2} - 1\]
			\end{prop}
			\begin{proof} This will be proven with induction and a base case of $n=1$.
				\begin{enumerate}
					\item[(1)] For $n=1$, this holds true as $1 = 2 - 1$.
					
					\item[(2)] Suppose the proposition is true for a positive integer $k$,  
					 \begin{align*}
						\sum_{i=1}^k F_i & = F_{k+2} - 1
						\intertext{For the next $k$ in sequence,}
						\sum_{i=1}^{k+1} F_i & = \sum_{i=1}^k F_i + F_{k+1} \\
							& = \left( F_{k+2} - 1 \right) + F_{k+1} && \text{(ind. hyp.)}
					\intertext{By the definition the Fibonacci sequence, the RHS can be rewritten as the next in sequence as}
						\sum_{i=1}^{k+1} F_i & = F_{(k+1) + 1} - 1
					\end{align*}
					Therefore this proposition is true for all $F_n$ in the Fibonacci sequence.
				\end{enumerate}
			\end{proof}
		\end{minipage}
	
		\item \begin{minipage}[t]{\linewidth}
			\begin{prop} For all integers $n \ge 1$, 
				\[ F_n = \frac{ \varphi^n - \psi^n }{\sqrt{5}} \]
				where $\varphi = \frac{1+ \sqrt{5}}{2}$ and $\psi = \frac{1 - \sqrt{5}}{2}$.
			\end{prop}
			\begin{proof} This will be proven with induction and a base case of $n=1$ and $n=2$.
				\begin{enumerate}
					\item[(1)] For $n=1$, $F_n = 1$ and the RHS fraction is \begin{align*}
						\frac{(1 + \sqrt{5}) - (1 - \sqrt{5})}{2 \sqrt{5}} = 1
						\intertext{For $n=2$, $F_n = 1$ and the RHS is}
						\frac{(1 + \sqrt{5})^2 - (1 - \sqrt{5})^2}{4\sqrt{5}} = 1
					\end{align*}
					\item[(2)] Suppose the proposition is true for $S_k$. This means it is true that \begin{align*}
						F_s & = \frac{\varphi^k - \psi^k}{\sqrt{5}}
						\intertext{Next, we will check this to be true for $k+1$. By the definition of the Fibonacci sequence,}
						F_{k+1} & = F_{k} + F_{k-1} \\
							& = \frac{1}{\sqrt{5}} \left[
								\left(\varphi^k - \psi^{k}\right)
								+ \left(\varphi^{k-1} - \psi^{k-1}\right)
							\right]\\
							& = \frac{1}{\sqrt{5}} \left[ \varphi^k \bigg( \underbrace{ 1 + \varphi^{-1} }_{\varphi}\bigg) - \psi^{k} \bigg(\underbrace{1 + \psi^{k-1}}_{\psi}\bigg)\right] \\
							& = \frac{\varphi^{k+1} - \psi^{k+1}}{\sqrt{5}}
					\end{align*}
					As this is true for the $k+1$ term, it must be true for all $n \ge 1$.
				\end{enumerate}
			\end{proof}
		\end{minipage}
		
	\end{enumerate}
\end{document}